\documentclass[12pt]{article}
\usepackage{amsmath}
\usepackage{amssymb}

\begin{document}

\begin{itemize}
	\item \( T_{p,q} (a ,\ b) = (bq + aq + ap ,\ bp + aq ) \)
	\item \( T_{p,q} (bq + aq + ap ,\ bp + aq ) = ( (bp + aq) q +
		(bq + aq + ap) q + (bq + aq + ap) p ,\ pe (bp + aq) p +
		(bq + aq + ap) q )) = (bq\prime + aq\prime + ap\prime ,\
		bp\prime + aq\prime)\)
	\item If we expand the first parameter:

		\[ bpq + aqq + bqq + aqq + apq + bpq + apq + app\]
		\[ = b q\prime + a q\prime + a p\prime \]

		Which can be written in the form:

		\[ b (2pq + qq) + a (2pq + qq) + a (pp + qq) \]
		\[ = b q\prime + a q\prime + a p\prime \] 

		Therefore:

		\[ p = (p ^2 + q ^2) \] 
		\[ q = (2pq + q ^2) \] 

		As desired.

\end{itemize}

\end{document}
